bedrock2/src/BasicC64Semantics.v
@@ -1,0 +1,20 @@
+Require Import bedrock2.BasicC64Syntax bedrock2.Semantics.
+Require bedrock2.String.
+Require bbv.Word.
+
+Instance parameters : parameters := {|
+  syntax := StringNames.Syntax.make BasicC64Syntax.parameters;
+  word := Word.word 64;
+  word_zero := Word.wzero 64;
+  word_succ := Word.wplus (Word.wone 64);
+  word_test w := if Word.weq (Word.wzero 64) w then false else true;
+  word_of_Z w := Some (Word.ZToWord 64 w);
+  interp_binop := _;
+  byte := Word.word 8;
+  combine _ b w := Word.wor (Word.wlshift' w 8) (Word.zext b (64-8));
+  split _ w := (Word.split1 8 (64-8) w, Word.zext (Word.split2 8 (64-8) w) 8);
+  mem := _;
+  locals := _;
+  funname_eqb := String.eqb;
+|}.
+Admitted.
