bedrock2/src/Notations.v
@@ -1,0 +1,18 @@
+Require Import bedrock2.Macros.
+
+Notation "' x <- a | y ; f" :=
+  (match a with
+   | x => f
+   | _ => y
+   end)
+  (right associativity, at level 70, x pattern).
+
+Notation "'bind_ex' x <- a ; f" :=
+  (subst! a for a' in exists x, a' x /\ f)
+  (only parsing, right associativity, at level 60, f at level 200).
+Notation "'bind_ex_Some' x <- a ; f" :=
+  (subst! a for a' in exists x, a' = Some x /\ f)
+  (only parsing, right associativity, at level 60, f at level 200).
+Notation "'bind_eq' x <- a ; f" :=
+  (subst! a for a' in forall x, x = a' -> f)
+  (only parsing, right associativity, at level 60, f at level 200).
