bedrock2/src/Semantics.v
@@ -1,0 +1,45 @@
+Require Import bedrock2.Macros bedrock2.Notations bedrock2.Syntax bedrock2.Map.
+Require Import Coq.ZArith.BinIntDef.
+
+Class parameters := {
+  syntax :> Syntax.parameters;
+
+  word : Type;
+  word_zero : word;
+  word_succ : word -> word;
+  word_test : word -> bool;
+  word_of_Z : BinNums.Z -> option word;
+  interp_binop : bopname -> word -> word -> word;
+
+  byte : Type;
+  (* nat included for conceptual completeness, only middle-endian would use it *)
+  combine : nat -> byte -> word -> word;
+  split : nat -> word -> byte * word;
+
+  mem :> map word byte;
+  locals :> map varname word;
+
+  funname_eqb : funname -> funname -> bool
+}.
+
+Section semantics.
+  Context {pp : unique! parameters}.
+  
+  Fixpoint load (sz : nat) (m:mem) (a:word) : option word :=
+    match sz with
+    | O => Some word_zero
+    | S sz =>
+      'Some b <- map.get m a             | None;
+      'Some w <- load sz m (word_succ a) | None;
+       Some (combine sz b w)
+    end.
+  Fixpoint store (sz : nat) (m:mem) (a v:word) : option mem :=
+    match sz with
+    | O => Some m
+    | S sz =>
+      let '(b, w) := split sz v in
+      'Some _ <- map.get m a | None;
+      store sz (map.put m a b) (word_succ a) w
+    end.
+  Definition trace := list ((mem * actname * list word) * (mem * list word)).
+End semantics.
